@prefix rdf:        <http://www.w3.org/1999/02/22-rdf-syntax-ns#> .
@prefix rdfs:         <http://www.w3.org/2000/01/rdf-schema#> .
@prefix owl:         <http://www.w3.org/2002/07/owl#> .
@prefix foaf:         <http://xmlns.com/foaf/0.1/> .
@prefix dc:         <http://purl.org/dc/terms/> .
@prefix xsd:         <http://www.w3.org/2001/XMLSchema#> .
@prefix skos:         <http://www.w3.org/2004/02/skos/core#> .
@prefix hxl:         <http://hxl.humanitarianresponse.info/ns-2012-06-12/#> . # update

<http://hxl.humanitarianresponse.info/ns-2012-06-12/> a owl:Ontology ;   # update
        dc:date "2012-06-20"^^xsd:date ;                                                                 # update
        dc:creator hxl:carsten , hxl:cj , hxl:minu ;
        dc:title "Humanitarian eXchange Language (HXL) Situation and Response Standard"@en ;
        dc:abstract "<p>Draft specification of the Humanitarian eXchange Language (HXL) standard. This vocabulary specification is currently <b>under development</b> and may change at any time without notice.</p> <p>The porpuse of HXL is to facilitate data exchange within the humanitarian domain. It provides a core domain model that has been created bottom-up by inspecting a broad range of systems in use with different humanitarian organisations. As needs vary widely across organisations in this domain, this vocabulary does <em>not</em> intend to be complete; in fact, it is the smallest common denominator. Any organisations that wish to publish <em>full</em> exports of their data can do so by extending this domain model with application- or organisation-specific models that reflect their internal data models (which may already be formalised in an XML schema or database schema).</p>"@en ;
        dc:license "We still need to decide under which license this vocabulary should be published."@en ;
        dc:versionOf <http://hxl.humanitarianresponse.info> ;
        rdfs:seeAlso "For further information about the HXL project, see <a href='https://sites.google.com/site/hxlproject/'>https://sites.google.com/site/hxlproject/</a>."@en ;
        dc:replaces <http://hxl.humanitarianresponse.info/ns-2012-05-16/> ; # update -> previous version 
        skos:changeNote "Changes compared to the previous version:<ol><li>Addition of <a href='#AgeGroupSet'>Age Group Set</a>, <a href='AdminDatasetVersion'>Administrative Units Dataset Version</a>, and <a href='DisplacedLocationTypeSet'>Displaced Persons Location Type Set</a> to allow for versioning of these references for different emergencies or changes over time.</li><li>Classes and properties not required for the HXL Phase 2 development were removed.  The Humanitarian Profile and cross-cutting components (date/time, geolocation, metadata, etc.) remain.</li><li>The <em>provenanceInfo</em> property was replaced by <a href='#source'>source</a> and <a href='#method'>method</a> for compliance with the humanitarian profile.</li></ol>" . 


# define the different vocabulary sections for vocabulary management 
hxl:humanitarianProfileSection a hxl:vocabularySection ;
        rdfs:comment "This section of the vocabulary defines the humanitarian profile standard which includes classes for describing populations affected by an emergency."@en ;
dc:title "Humanitarian Profile Section"@en .		
hxl:geolocationSection a hxl:vocabularySection ;
        rdfs:comment "This section of the vocabulary defines the geolocation standard. The <a href='hxl-geolocation-standard-draft.pdf'>draft HXL geolocation standard</a> contains a detailed description of how to use the classes and properties."@en ;
dc:title "Geolocation Section".
hxl:datetimeSection a hxl:vocabularySection ; 
        rdfs:comment "This section of the vocabulary defines the date/time standard. The <a href='hxl-datetime-standard-draft.pdf'>draft HXL date/time standard</a> contains a detailed description of how to use the classes and properties."@en         ;
dc:title "Date/Time Section".
hxl:situationSection a hxl:vocabularySection ;
        rdfs:comment "This section of the vocabulary defines the standards for situations and emergencies."@en ;
dc:title "Situation Section".
hxl:responseSection a hxl:vocabularySection ;
        rdfs:comment "This section of the vocabulary defines the standards for response activities."@en ;
dc:title "Response Section".
#hxl:shelterClusterSection a hxl:vocabularySection ;
#        rdfs:comment "This section of the vocabulary defines the standards for the shelter cluster."@en ;
#dc:title "Shelter Cluster Section".
#hxl:washClusterSection a hxl:vocabularySection ;
#        rdfs:comment "This section of the vocabulary defines the standards for the WASH cluster."@en ;
#dc:title "WASH Cluster Section".
hxl:metadataSection a hxl:vocabularySection ;
        rdfs:comment "This section of the vocabulary defines the standards for metadata about a set of HXL data that is being exchanged."@en ;
dc:title "Metadata Section".
                
hxl:carsten foaf:name "Carsten Keßler" ;
        foaf:mbox "me@carsten.io" ;
        foaf:homepage <http://carsten.io> .

hxl:cj foaf:name "CJ Hendrix" ;
        foaf:mbox "hendrix.cj@gmail.com" .

hxl:minu foaf:name "Minu Limbu" ;
        foaf:mbox "minulimbu@gmail.com" .
                
hxl:Situation
        a rdfs:Class ;
        rdfs:isDefinedBy hxl:situationSection;
        skos:prefLabel "Situation"@en ;
        rdfs:comment "Generic situation."@en.          # eventually add more languages ?
        
hxl:AdminUnit
        a rdfs:Class ;
        rdfs:isDefinedBy hxl:geolocationSection;
        skos:prefLabel "Administrative Unit"@en ;
        rdfs:subClassOf hxl:Feature ;
        rdfs:comment "Administrative units can include coutries, regions, cities, etc. The hierarchy of administrative units can vary from country to country."@en .        

hxl:PopulatedPlace
        a rdfs:Class ;
        rdfs:isDefinedBy hxl:geolocationSection;
        skos:prefLabel "Populated Place"@en ;
        rdfs:subClassOf hxl:AdminUnit ;
rdfs:comment "Lowest-level administrative unit, such as a town or settlement."@en .
        
hxl:Country
        a rdfs:Class ;
        rdfs:isDefinedBy hxl:geolocationSection;
        skos:prefLabel "Country"@en ;
        rdfs:subClassOf hxl:AdminUnit ;
rdfs:comment "Highest-level administrative unit (level 0)."@en .

hxl:AdminUnitLevel
        a rdfs:Class ;
        rdfs:isDefinedBy hxl:geolocationSection;
        skos:prefLabel "Administrative Unit Level"@en ;
        rdfs:comment "The specific administrative unit levels can vary from country to country. Administrative Unit Level 0 is a country – in this case, hxl:Country should be used."@en .

hxl:AffectedPopulation
        a rdfs:Class ;
        rdfs:isDefinedBy hxl:humanitarianProfileSection ;
        skos:prefLabel "Affected Population"@en ;
        rdfs:subClassOf hxl:Population ;
        rdfs:comment "The population affected by an emergency.<br /><small>Term origin: Humanitarian Profile (<em>Affected</em>);</small>"@en .        

hxl:Population
        a rdfs:Class ;
        rdfs:isDefinedBy hxl:humanitarianProfileSection ;
        skos:prefLabel "Population"@en ;
        rdfs:subClassOf foaf:Group ;
        rdfs:comment "Generic class for any kind of population. Example: Total population, affected population etc; use the subclasses for the data annotation."@en .

hxl:TotalPopulation
        a rdfs:Class ;
        rdfs:isDefinedBy hxl:humanitarianProfileSection ;
        skos:prefLabel "Total Population"@en ;
        rdfs:subClassOf hxl:Population ;
        rdfs:comment "Total population for a given administrative unit or geographic area. Instances can be created to make statements about this population."@en .

hxl:AgeGroup
        a rdfs:Class ;
        rdfs:isDefinedBy hxl:humanitarianProfileSection ;
        skos:prefLabel "Age Group"@en ;
        rdfs:comment "Generic class for age groups; instances should be created for actual age groups. Example: <em>Children under 5</em>. " .
        
hxl:Casualty
        a rdfs:Class ;
        rdfs:isDefinedBy hxl:humanitarianProfileSection ;
        rdfs:subClassOf hxl:AffectedPopulation ;
        skos:prefLabel "Casualty"@en ;
        rdfs:comment "Examples: <em>Injured</em> or <em>dead</em>.<br /><small>Term origin: ACAPS DSS, Humanitarian Profile.</small>" .
        
hxl:Dead
        a rdfs:Class ;
        rdfs:isDefinedBy hxl:humanitarianProfileSection ;
        skos:prefLabel "Dead"@en ;
        skos:altLabel "Death"@en ;
        rdfs:subClassOf hxl:Casualty ;
        owl:disjointWith hxl:Injured ;
        rdfs:comment "A (reported) death.<br /><small>Term origin: ACAPS DSS, HPM Ethiopia, Shelter Cluster, Humanitarian Profile (<em>Dead</em>).</small>" .
        
hxl:Displaced
        a rdfs:Class ;
        rdfs:isDefinedBy hxl:humanitarianProfileSection ;
        skos:prefLabel "Displaced"@en ;
        skos:altLabel "Displacement"@en ;
        rdfs:subClassOf hxl:AffectedPopulation ;
        rdfs:comment "Refers to internally displaced persons, refugees, and others of concern.<br /><small>Term origin: Humanitarian Profile, ACAPS DSS (<em>Displacement</em>)</small>" ;
owl:disjointWith hxl:NonDisplaced .

hxl:currentLocation 
        a rdf:Property, owl:ObjectProperty ;
        rdfs:isDefinedBy hxl:humanitarianProfileSection ;
        skos:prefLabel "current location"@en;
        rdfs:domain hxl:Population ;
        rdfs:range hxl:Feature ;
rdfs:comment "The current location of the population being reported should be given at the level of geographic detail agreed by the IM Network using the Administrative Boundaries and Populated Places Common Operational Datasets. Organizations reporting Humanitarian Profile numbers should be encouraged to use the p-code system for unambiguous location reporting.<br /><small>Term origin: Humanitarian profile.</small>" .

hxl:includes 
        a rdf:Property, owl:ObjectProperty ;
        rdfs:isDefinedBy hxl:humanitarianProfileSection ;
        skos:prefLabel "includes"@en;
        rdfs:domain hxl:Population ;
        rdfs:range hxl:Population ;
rdfs:comment "Property to state that one population is part of another one (e.g. the population at camp XY includes a certain age group with a number of persons in them).<br /><small>Term origin: Humanitarian profile.</small>" .

hxl:placeOfOrigin 
        a rdf:Property, owl:ObjectProperty ;
        rdfs:isDefinedBy hxl:humanitarianProfileSection ;
        skos:prefLabel "place of origin"@en;
        rdfs:domain hxl:Displaced ;
        rdfs:range hxl:Feature ;
rdfs:comment "This attribute only applies to Displaced and its subclasses. It should include p-coded location from which the population being reported moved as a result of the emergency.<br /><small>Term origin: Humanitarian profile.</small>" .

hxl:nationality 
        a rdf:Property, owl:ObjectProperty ;
        rdfs:isDefinedBy hxl:humanitarianProfileSection ;
        skos:prefLabel "nationality"@en;
        rdfs:domain hxl:Population ;
        rdfs:range hxl:Country ;
rdfs:comment "This item generally only applies to populations displaced across international borders and contains the nationality of the population being reported.<br /><small>Term origin: Humanitarian profile.</small>" .

hxl:NonDisplaced
        a rdfs:Class ;
        rdfs:isDefinedBy hxl:humanitarianProfileSection ;
        skos:prefLabel "Non-Displaced"@en ;
        rdfs:subClassOf hxl:AffectedPopulation ;
        rdfs:comment "Refers to the part of the affected population that is not displaced (i.e., host or non-host);.<br /><small>Term origin: Humanitarian Profile.</small>" ;
owl:disjointWith hxl:Displaced .

hxl:HostPopulation
        a rdfs:Class ;
        rdfs:isDefinedBy hxl:humanitarianProfileSection ;
        skos:prefLabel "Host population"@en ;
        rdfs:subClassOf hxl:NonDisplaced ;
        rdfs:comment "Persons who are part of a host community or family receiving affected people. Due to the stress placed on the host families and communities, they are considered part of the humanitarian caseload.<br /><small>Term origin: Humanitarian Profile.</small>" ;
owl:disjointWith hxl:NonHostPopulation .

hxl:NonHostPopulation
        a rdfs:Class ;
        rdfs:isDefinedBy hxl:humanitarianProfileSection ;
        skos:prefLabel "Non-host population"@en ;
        rdfs:subClassOf hxl:NonDisplaced ;
        rdfs:comment "People requiring immediate assistance during a period of emergency who have not moved from their homes or places of habitual residence.<br /><small>Term origin: Humanitarian Profile.</small>" ;
owl:disjointWith hxl:HostPopulation .

hxl:Emergency
        a rdfs:Class ;
        rdfs:isDefinedBy hxl:situationSection;        
        skos:prefLabel "Emergency"@en ;
        rdfs:subClassOf hxl:Situation ;
        rdfs:comment "<p>Any situation in which ... life or well-being ... will be threatened  unless immediate  and  appropriate   action  is  taken,  and  which demands   an   extraordinary   response   and   exceptional measures” (UNHCR Handbook for Emergencies)</p><p>A sudden crisis situation or event requiring immediate action (WART) </p><p>Any situation in which there is an exceptional and widespread threat to life, health or basic  subsistence,  that  is  beyond  the  coping  capacity  of individuals and the community”  (Oxfam GB Emergency Response Manual). </p><p>Where and when a disaster provokes an immediate, exceptional and widespread threat to life, health or basic subsistence, which overwhelms the coping capacity of individual and community, implying need of external assistance” (source: ACFIN Emergency module)</p><small>Term origin: CAP OPS, Pakistan SRF, ACAPS DSS, CERF, MIRA.</small>" .

hxl:GLIDEnumber
        a rdfs:Class ;
        rdfs:isDefinedBy hxl:situationSection;        
        skos:prefLabel "GLIDE number"@en ;
        rdfs:comment "Globally common Unique ID code for disasters. See <a href='http://glidenumber.net/glide/public/about.jsp'>about GLIDE</a>." .

hxl:Female
        a rdfs:Class ;
        rdfs:isDefinedBy hxl:humanitarianProfileSection ;
        skos:prefLabel "Female"@en;        
        rdfs:subClassOf hxl:Sex ;
        rdfs:comment "A woman/girl or group of women/girls.<br /><small>Term origin: CERF, EIMS Report.</small>" ;
owl:disjointWith hxl:Male , hxl:Intersex , hxl:MixedSex .

hxl:Male
        a rdfs:Class ;
        rdfs:isDefinedBy hxl:humanitarianProfileSection ;        
        skos:prefLabel "Male"@en;
        rdfs:subClassOf hxl:Sex ;
        rdfs:comment "A man/boy or group of men/boys.<br /><small>Term origin: CERF, EIMS Report.</small>" ;
owl:disjointWith hxl:Female , hxl:Intersex , hxl:MixedSex .     

hxl:Sex
        a rdfs:Class ;
        rdfs:isDefinedBy hxl:humanitarianProfileSection ;        
        skos:prefLabel "Sex"@en;
        rdfs:comment "Class to describe sex-specific issues, either at individual or group level.<br /><small>Term origin: MIRA, CCDI</small>" .

hxl:Response
        a rdfs:Class ;
        rdfs:isDefinedBy hxl:responseSection ;
        skos:prefLabel "Response"@en;
        rdfs:comment "Generic term for the collection of all activities that address the needs arising from an emergency.<br /><small>Term origin: ACAPS DSS, ACAPS DSS, MIRA, EDXL, CCDI (<em>Humanitarian Response</em>), CERF (<em>Humanitarian Response</em>)</small>" .

hxl:IDP
        a rdfs:Class ;
        rdfs:isDefinedBy hxl:humanitarianProfileSection  ;
        rdfs:subClassOf hxl:Displaced ;
        skos:prefLabel "Internally Displaced Person"@en;
        skos:altLabel "IDP"@en;
        owl:disjointWith hxl:Others ;
        owl:disjointWith hxl:RefugeesAsylumSeekers ;
        rdfs:comment "A group of internally displaced persons (IDPs).<br /><small>Term origin: Humanitarian Profile, CERF, HPM Ethiopia</small>" .

hxl:Others
        a rdfs:Class ;
        rdfs:isDefinedBy hxl:humanitarianProfileSection  ;
        rdfs:subClassOf hxl:Displaced ;
        skos:prefLabel "Others of Concern"@en;
        owl:disjointWith hxl:IDP ;
        owl:disjointWith hxl:RefugeesAsylumSeekers ;
        rdfs:comment "Persons who have been displaced by the emergency and form part of the humanitarian caseload, but do not fall into the IDP or refugees/asylum seekers categories.<br /><small>Term origin: Humanitarian Profile</small>" .

hxl:RefugeesAsylumSeekers
        a rdfs:Class ;
        rdfs:isDefinedBy hxl:humanitarianProfileSection  ;
        rdfs:subClassOf hxl:Displaced ;
        skos:prefLabel "Refugees and Asylum Seekers"@en;
        owl:disjointWith hxl:IDP ;
        owl:disjointWith hxl:Others ;
        rdfs:comment "A group of refugees and asylum seekers.<br /><small>Term origin: Humanitarian Profile</small>" .

hxl:Injured
        a rdfs:Class ;
        rdfs:isDefinedBy hxl:humanitarianProfileSection  ;
        rdfs:subClassOf hxl:Casualty ;
        skos:prefLabel "Injured"@en;
        owl:disjointWith hxl:Dead ;
        rdfs:comment "Indicates the Injured population.<br /><small>Term origin: ACAPS DSS, Humanitarian Profile, Shelter Cluster, HERAMS Checklist (<em>Injury</em>)</small>" .

hxl:Feature
        a rdfs:Class ;
        rdfs:isDefinedBy hxl:geolocationSection ;
        skos:prefLabel "Feature"@en;
        rdfs:subClassOf <http://www.w3.org/2003/01/geo/wgs84_pos#SpatialThing> ;
rdfs:comment "Any real-word phenomenon with spatial extent, i.e. size, shape, or position. " .

hxl:Geometry
        a rdfs:Class ;
        rdfs:isDefinedBy hxl:geolocationSection ;
        skos:prefLabel "Geometry"@en;
rdfs:comment "Abstract root class of the geometry. This class should not be instantiated; use any of the subclasses when creating actual geometries. " .

hxl:Point
        a rdfs:Class ;
        rdfs:isDefinedBy hxl:geolocationSection ;
        skos:prefLabel "Point"@en;
        rdfs:subClassOf hxl:Geometry;
rdfs:comment "A Point is a 0-dimensional geometric object and represents a single location in a two- or three-dimensional coordinate space." .

hxl:Line
        a rdfs:Class ;
        rdfs:isDefinedBy hxl:geolocationSection ;
        skos:prefLabel "Line String"@en;
        rdfs:subClassOf hxl:Geometry;
rdfs:comment "A LineString is a Curve with linear interpolation between Points. Each consecutive pair of Points defines a Line segment." .

hxl:Polygon
        a rdfs:Class ;
        rdfs:isDefinedBy hxl:geolocationSection ;
        skos:prefLabel "Polygon"@en;
        rdfs:subClassOf hxl:Geometry;
rdfs:comment "A Polygon is a planar Surface defined by 1 exterior boundary and 0 or more interior boundaries. Each interior boundary defines a hole in the Polygon." .

hxl:BoundingBox
        a rdfs:Class ;
        rdfs:isDefinedBy hxl:geolocationSection ;
        skos:prefLabel "Bounding Box"@en;
        rdfs:subClassOf hxl:Polygon;
rdfs:comment "A BoundingBox is a Polygon defined by 1 exterior boundary and 0 interior boundaries. The exterior boundary consists of 4 points arranged as a rectangle." .

hxl:Missing
        a rdfs:Class ;
        rdfs:isDefinedBy hxl:humanitarianProfileSection  ;
        skos:prefLabel "Missing"@en ;
        rdfs:subClassOf hxl:Casualty ;
        owl:disjointWith hxl:Dead ;
        rdfs:comment "Associated with <i>Missing Persons</i> as a major humanitarian concern in complex emergencies where many people go missing, causing anguish and uncertainty for their families and friends. See <em> ICRC </em>. <br /><small>Term origin: Humanitarian Profile.</small>" .

hxl:Organisation
        a rdfs:Class ;
        rdfs:isDefinedBy hxl:responseSection  ;
        rdfs:subClassOf foaf:Organisation ;
        skos:prefLabel "Organisation"@en ;
rdfs:comment "A humanitarian organisation.<br /><small>Term origin: IATI, CAP OPS, Pakistan SRF, EIMS Report, Shelter Cluster, Sigmah DB.</small>" .

hxl:GovernmentOrganisation
        a rdfs:Class ;
        rdfs:isDefinedBy hxl:responseSection  ;
        rdfs:subClassOf hxl:Organisation ;
        skos:prefLabel "Government organisation"@en ;
rdfs:comment "A government organisation.<br /><small>Term origin: FTS.</small>" .

hxl:InterGovernmentalOrganisation
        a rdfs:Class ;
        rdfs:isDefinedBy hxl:responseSection  ;
        rdfs:subClassOf hxl:Organisation ;
        skos:prefLabel "Inter-governmental organisation"@en ;
rdfs:comment "An inter-governmental organisation (IGOs) is an organization composed primarily of sovereign states (referred to as member states), or of other intergovernmental organizations.Example:  NATO, SAARC. <br /><small>Term origin: FTS.</small>" .

hxl:UNAgency
        a rdfs:Class ;
        rdfs:isDefinedBy hxl:responseSection  ;
        rdfs:subClassOf hxl:Organisation ;
        skos:prefLabel "UN agency"@en ;
rdfs:comment "Specialized agencies that carry out various functions on behalf of the United Nations. Example: WHO, WFP.An UN agency.<br /><small>Term origin: FTS.</small>"@en .

hxl:RedCrossRedCrescent
        a rdfs:Class ;
        rdfs:isDefinedBy hxl:responseSection ;
        rdfs:subClassOf hxl:Organisation ;
        skos:prefLabel "Red cross / red crescent"@en ;
rdfs:comment "Organisations under the world's largest humanitarian network  of International Red Cross and Red Crescent Movement.(source:IFRC )Organisation under red cross / red crescent.<br /><small>Term origin: FTS.</small>" .

hxl:NGO
        a rdfs:Class ;
        rdfs:isDefinedBy hxl:responseSection ;
        rdfs:subClassOf hxl:Organisation ;
        skos:prefLabel "NGO"@en ;
        skos:altLabel "Non-governmental organisation"@en ;        
rdfs:comment "A non-governmental organization (NGO) is a nonprofit, voluntary citizens' group that operates independently from any government on a local, national or international level. Example:  Wolrd Vision International, ACF, Oxfam.<small>Term origin: FTS.</small>"@en .

hxl:PrivateOrganisation
        a rdfs:Class ;
        rdfs:isDefinedBy hxl:responseSection ;
        rdfs:subClassOf hxl:Organisation ;
        skos:prefLabel "Private organisation / foundation"@en ;
rdfs:comment "is a self-sustaining special interest groups (like business firms) with activities mor enclined towards profit making. <small>Term origin: FTS.</small>"@en .

hxl:BilateralOrganisation
        a rdfs:Class ;
        rdfs:isDefinedBy hxl:responseSection ;
        rdfs:subClassOf hxl:Organisation ;
        skos:prefLabel "Bilateral organisation"@en ;
rdfs:comment "A bilateral organization is a government agency or nonprofit organization based in a single country while the agency provides aid, including medical aid or disaster relief, for people in other countries. Example:  DFID, AusAID, USAID. <small>Term origin: FTS.</small>"@en .

hxl:ReportingPeriod
        a rdfs:Class ;
        rdfs:isDefinedBy hxl:datetimeSection ;
        skos:prefLabel "Reporting Period"@en;
        rdfs:subClassOf dc:PeriodOfTime ;
        rdfs:comment "The time frame that a report covers.<br /><small>Term origin: Sigmah DB.</small>" .

hxl:TotalPopulation
        a rdfs:Class ;
        rdfs:isDefinedBy hxl:humanitarianProfileSection  ;
        rdfs:subClassOf hxl:Population ;
        skos:prefLabel "Total Population"@en;
rdfs:comment "The total population for an administrative unit. Example: A region.<br /><small>Term origin: Shelter Cluster.</small>" .

hxl:DataContainer
        a rdfs:Class ;
        rdfs:isDefinedBy hxl:metadataSection ;
        skos:prefLabel "Data container"@en;
rdfs:comment "This is the <em>container</em> element for to attach any metadata to. Any HXL file has to include exactly one data container element and make all metadata statements about this container. When loading the file into the triple store, a new named graph will be created that inherits the metadata from this container." .

hxl:ApprovalLevel
        a rdfs:Class ;
        rdfs:isDefinedBy hxl:metadataSection ;
        skos:prefLabel "Approval level"@en;
rdfs:comment "Instance of this class define fixed levels of approval. Example:  in the WHO system, there could be three levels: region, country, and world." .

hxl:organisationHomepage
        a rdf:Property, owl:ObjectProperty ;
        rdfs:isDefinedBy hxl:responseSection ;
        skos:prefLabel "organisation homepage" ;
        rdfs:subPropertyOf foaf:homepage ;
        rdfs:comment "States the website of a given organisation. <small>Term origin: FTS.</small>" ;                
        rdfs:domain hxl:Organisation ;
rdfs:range foaf:Document .

hxl:orgName
        a rdf:Property, owl:DataProperty ;
        rdfs:isDefinedBy hxl:responseSection ;
        skos:prefLabel "organisation name" ;
        rdfs:comment "States the name of the organisation. <small>Term origin: FTS.</small>" ;                
        rdfs:domain hxl:Organisation ;
rdfs:range rdfs:Literal .

hxl:abbreviation
        a rdf:Property, owl:DataProperty ;
        rdfs:isDefinedBy hxl:responseSection ;
        skos:prefLabel "organisation abbreviation" ;
        rdfs:comment "Indicates the abbreviation of the Organisation. <small>Term origin: FTS.</small>" ;                
        rdfs:domain hxl:Organisation ;
rdfs:range rdfs:Literal .

hxl:orgNativeName
        a rdf:Property, owl:DataProperty ;
        rdfs:isDefinedBy hxl:responseSection ;
        skos:prefLabel "native organisation name" ;
        rdfs:comment "Specifies the native name of the organisation. <small>Term origin: FTS.</small>" ;                
        rdfs:domain hxl:Organisation ;
rdfs:range rdfs:Literal .

hxl:orgDisplayName
        a rdf:Property, owl:DataProperty ;
        rdfs:isDefinedBy hxl:responseSection ;
        skos:prefLabel "organisation name for display" ;
        rdfs:comment "Indicates the organisation name that is most commonly used and displayed.  <small>Term origin: FTS.</small>" ;                
        rdfs:domain hxl:Organisation ;
rdfs:range rdfs:Literal .

hxl:reportedBy
        a rdf:Property , owl:ObjectProperty ;        
        rdfs:isDefinedBy hxl:metadataSection ;
        skos:prefLabel "reported by"@en ;
        rdfs:comment "The reporting person or organization - not necessarily involved in the aid activity itself, though in practice it often will be a donor or appealing agency.  <br /><small>Term origin: IATI.</small>"@en ;
        rdfs:domain hxl:DataContainer ;        
rdfs:range foaf:Agent .

hxl:approvedBy
        a rdf:Property , owl:ObjectProperty ;        
        rdfs:isDefinedBy hxl:metadataSection ;
        skos:prefLabel "approved by"@en ;
        rdfs:comment "Link from a container to the person or organisation who has 'lifted' it to the current approvalLevel."@en ;
        rdfs:domain hxl:DataContainer ;        
rdfs:range foaf:Agent .

hxl:approvedAtLevel
        a rdf:Property , owl:ObjectProperty ;        
        rdfs:isDefinedBy hxl:metadataSection ;
        skos:prefLabel "approved at level"@en ;
        rdfs:comment "A container can have approval at different levels, which may in turn indicate for which kind of analyses the data in this container is fit.</em>"@en ;
        rdfs:domain hxl:DataContainer ;        
rdfs:range hxl:ApprovalLevel .

hxl:containsPrimaryData
        a rdf:Property , owl:DataProperty ;        
        rdfs:isDefinedBy hxl:metadataSection ;
        skos:prefLabel "contains primary data"@en ;
        rdfs:comment "A container can contain primary data, secondary data, or both.</em>"@en ;
rdfs:domain hxl:DataContainer ;        
rdfs:range rdfs:Literal .

hxl:containsSecondaryData
        a rdf:Property , owl:DataProperty ;        
        rdfs:isDefinedBy hxl:metadataSection ;
        skos:prefLabel "contains secondary data"@en ;
        rdfs:comment "A container can contain primary data, secondary data, or both.</em>"@en ;
rdfs:domain hxl:DataContainer ;        
rdfs:range rdfs:Literal .

hxl:affectedBy
        a rdf:Property , owl:ObjectProperty ;
        rdfs:isDefinedBy hxl:humanitarianProfileSection  ;
        skos:prefLabel "affected by"@en ;
        rdfs:comment "States that a Population is affacted by an Emergency."@en ;
        rdfs:domain hxl:AffectedPopulation ;
rdfs:range hxl:Emergency .

hxl:affects owl:inverseOf hxl:affectedBy .

hxl:fromAge        
        a rdf:Property , owl:DataProperty ;
        rdfs:isDefinedBy hxl:humanitarianProfileSection  ;
        skos:prefLabel "from age"@en ;
        rdfs:comment "Specifies the bottom of an age range for an AgeGroup (in years)." ;
        rdfs:domain hxl:AgeGroup ;
rdfs:range rdfs:Literal .

hxl:toAge        
        a rdf:Property , owl:DataProperty ;
        rdfs:isDefinedBy hxl:humanitarianProfileSection  ;
        skos:prefLabel "to age"@en ;
        rdfs:comment "Specifies the top of an age range for an AgeGroup (in years)." ;
        rdfs:domain hxl:AgeGroup ;
rdfs:range rdfs:Literal .

hxl:atLocation
        a rdf:Property, owl:ObjectProperty ;
        rdfs:isDefinedBy hxl:geolocationSection ;
        skos:prefLabel "at Location"@en ;
        rdfs:subPropertyOf dc:spatial ; 
        rdfs:comment "Specififes the location for things like emergencies, projects, or camps."@en ;
        rdfs:domain hxl:Situation ; 
rdfs:range hxl:Feature .

hxl:locationOf owl:inverseOf hxl:atLocation .

hxl:atLevel
        a rdf:Property, owl:ObjectProperty ;
        rdfs:isDefinedBy hxl:geolocationSection ;
        skos:prefLabel "at level"@en;
        rdfs:comment "Specifies the level for an administrative unit.";
        rdfs:domain hxl:AdminUnit;
rdfs:range hxl:AdminUnitLevel .

hxl:levelOf owl:inverseOf hxl:atLevel .

hxl:inAdminUnit
        a rdf:Property, owl:ObjectProperty, owl:TransitiveProperty ;
        rdfs:isDefinedBy hxl:geolocationSection ;
        skos:prefLabel "in administrative unit"@en;
        rdfs:comment "Specifies direct containment between two administrative units. This property should only be used between administrative units that directly contain each other, i.e., when the administrative unit level of the containing unit is the level of the contained unit plus 1.";
        rdfs:domain hxl:AdminUnit;
rdfs:range hxl:AdminUnit .

hxl:hasGeometry
        a rdf:Property, owl:ObjectProperty ;
        rdfs:isDefinedBy hxl:geolocationSection ;
        skos:prefLabel "has geometry"@en ;
        rdfs:comment "Relates a feature to its geometry."@en ;
        rdfs:domain hxl:Feature ;
rdfs:range hxl:Geometry .

hxl:adminUnitLevelNumber
        a rdf:Property, owl:DataProperty ;
        rdfs:isDefinedBy hxl:geolocationSection ;
        skos:prefLabel "administrative unit level number"@en ;
        rdfs:comment "The number for this administrative unit level; e.g. 0 for country, 1 for state, etc."@en ;
        rdfs:domain hxl:AdminUnitLevel ;
rdfs:range rdfs:Literal .

hxl:adminUnitLevelTitle
        a rdf:Property , owl:DataProperty ;
        rdfs:isDefinedBy hxl:geolocationSection ;
        skos:prefLabel "administrative unit level title"@en ;
        rdfs:comment "The title for this administrative unit level; e.g. <em>state</em> or <em>city district</em>."@en ;
        rdfs:domain hxl:AdminUnitLevel ;
rdfs:range rdfs:Literal .

hxl:adminUnitLevelCountry
        a rdf:Property, owl:ObjectProperty ;
        rdfs:isDefinedBy hxl:geolocationSection ;
        skos:prefLabel "administrative unit level title"@en ;
        rdfs:comment "Relates an administrative unit level to the country (or countries) that it can be used in."@en ;
        rdfs:domain hxl:AdminUnitLevel ;
rdfs:range hxl:Country .

hxl:isGeometryOf owl:inverseOf hxl:hasGeometry .

hxl:asWKT
        a rdf:Property, owl:DataProperty ;
        rdfs:isDefinedBy hxl:geolocationSection ;
        skos:prefLabel "as WKT"@en ;
        rdfs:comment "A geometry serialised as WKT. Note that the WKT serialisation contains the spatial reference system (SRS), as specified in the <a href='http://portal.opengeospatial.org/files/?artifact_id=25355'>OGC Simple Feature standard</a>. If no SRS is given, HXL uses WGS 84 as the standard SRS."@en ;
        rdfs:domain hxl:Geometry ;
rdfs:range rdfs:Literal .

hxl:equals
        a rdf:Property, owl:ObjectProperty, owl:SymmetricProperty ;
        rdfs:isDefinedBy hxl:geolocationSection ;
        skos:prefLabel "equals"@en ;
        rdfs:comment "Topological relation. States that two geometries are equal."@en ;
        rdfs:domain hxl:Geometry ;
rdfs:range hxl:Geometry .

hxl:intersects
        a rdf:Property, owl:ObjectProperty ;
        rdfs:isDefinedBy hxl:geolocationSection ;
        skos:prefLabel "intersects"@en ;
        rdfs:comment "Topological relation. States that one geometry intersects another one. "@en ;
        rdfs:domain hxl:Geometry ;
rdfs:range hxl:Geometry .

hxl:touches
        a rdf:Property, owl:ObjectProperty, owl:SymmetricProperty ;
        rdfs:isDefinedBy hxl:geolocationSection ;
        skos:prefLabel "touches"@en ;
        rdfs:comment "Topological relation. States that one geometry touches another one. "@en ;
        rdfs:domain hxl:Geometry ;
rdfs:range hxl:Geometry .


hxl:crosses
        a rdf:Property, owl:ObjectProperty, owl:TransitiveProperty ;
        rdfs:isDefinedBy hxl:geolocationSection ;
        skos:prefLabel "crosses"@en ;
        rdfs:comment "Topological relation. States that one geometry crosses another one. "@en ;
        rdfs:domain hxl:Geometry ;
rdfs:range hxl:Geometry .

hxl:within
        a rdf:Property, owl:ObjectProperty, owl:TransitiveProperty ;
        rdfs:isDefinedBy hxl:geolocationSection ;
        skos:prefLabel "within"@en ;
        rdfs:comment "Topological relation. States that one geometry is within another one. "@en ;
        rdfs:domain hxl:Geometry ;
rdfs:range hxl:Geometry .

hxl:contains
        a rdf:Property, owl:ObjectProperty, owl:TransitiveProperty ;
        rdfs:isDefinedBy hxl:geolocationSection ;
        skos:prefLabel "contains"@en ;
        rdfs:comment "Topological relation. States that one geometry contains another one. "@en ;
        rdfs:domain hxl:Geometry ;
rdfs:range hxl:Geometry .

hxl:overlaps
        a rdf:Property, owl:ObjectProperty, owl:TransitiveProperty ;
        rdfs:isDefinedBy hxl:geolocationSection ;
        skos:prefLabel "overlaps"@en ;
        rdfs:comment "Topological relation. States that one geometry overlaps another one. "@en ;
        rdfs:domain hxl:Geometry ;
rdfs:range hxl:Geometry .

hxl:near
        a rdf:Property, owl:ObjectProperty, owl:SymmetricProperty ;
        rdfs:isDefinedBy hxl:geolocationSection ;
        skos:prefLabel "near"@en ;
        rdfs:comment "Topological relation. States that one geometry is near another one. "@en ;
        rdfs:domain hxl:Geometry ;
rdfs:range hxl:Geometry .

hxl:hasGLIDEnumber
        a rdf:Property, owl:ObjectProperty ;
        rdfs:isDefinedBy hxl:situationSection ;
        skos:prefLabel "has GLIDE number"@en ;
        rdfs:comment "Assigns the GLIDE number to an Emergency."@en ;
        rdfs:domain hxl:Emergency ;
rdfs:range hxl:GLIDEnumber .

hxl:count
        a rdf:Property, owl:DataProperty ;
        rdfs:isDefinedBy hxl:situationSection ;
        skos:prefLabel "count"@en ;
rdfs:comment "Property to count people, things, etc. Subproperties should be used if possible to clarify what has been counted."@en .

hxl:personCount
        a rdf:Property, owl:DataProperty ;
        rdfs:isDefinedBy hxl:humanitarianProfileSection ;
        skos:prefLabel "person count"@en ;
        rdfs:subPropertyOf hxl:count ;
        rdfs:comment "The number of persons in a population. The range is intentionally not restricted to numeric values, so that rough numbers or estimates are supported."@en ;
        rdfs:domain hxl:Population ;
rdfs:range rdfs:Literal .

hxl:householdCount
        a rdf:Property, owl:DataProperty ;
        rdfs:isDefinedBy hxl:humanitarianProfileSection ;
        skos:prefLabel "household count"@en ;
        rdfs:subPropertyOf hxl:count ;
        rdfs:comment "The number of people in a population. The range is intentionally not restricted to numeric values, so that rough numbers or estimates are supported."@en ;
        rdfs:domain hxl:Population ;
rdfs:range rdfs:Literal .

hxl:populationDescription
        a rdf:Property, owl:DataProperty ;
        rdfs:isDefinedBy hxl:humanitarianProfileSection ;
        skos:prefLabel "population description"@en ;
        rdfs:comment "A description of this population."@en ;
        rdfs:domain hxl:Population ;
rdfs:range rdfs:Literal .

hxl:source
        a rdf:Property, owl:ObjectProperty ;
        rdfs:isDefinedBy hxl:humanitarianProfileSection ;
        skos:prefLabel "source"@en ;
        rdfs:comment "The organization(s) providing the information. Note that in some cases, if the source is the same for all records, this item could be reported as metadata for the dataset rather than for each record.<br /><small>Source: Humanitarian profile.</small>"@en ;
        rdfs:domain hxl:Population ;
rdfs:range hxl:Organisation .

hxl:method
        a rdf:Property, owl:DataProperty ;
        rdfs:isDefinedBy hxl:humanitarianProfileSection ;
        skos:prefLabel "method"@en ;
        rdfs:comment "The method by which the Number of Persons was derived. Note that in some cases, if the method is the same for all records, this item could be reported as metadata for the dataset rather than for each record.<br /><small>Source: Humanitarian profile.</small>"@en ;
        rdfs:domain hxl:Population ;
rdfs:range rdfs:Literal .

hxl:commonTitle
        a rdf:Property, owl:DataProperty ;
        rdfs:isDefinedBy hxl:situationSection ;
        skos:prefLabel "common title"@en ;
        rdfs:comment "A commonly use title/name for an emergency."@en ;
        rdfs:domain hxl:Situation ;
rdfs:range rdfs:Literal .

# -- some stuff copied from other vocabs for completeness:

dc:PeriodOfTime
        a rdfs:Class , owl:Class ;
        rdfs:isDefinedBy hxl:datetimeSection ;
skos:prefLabel "dc:PeriodOfTime" .

hxl:situationDescription  #may want to link this to dbpedia article for major emergencies
        a rdf:Property , owl:DataProperty ;
        rdfs:subPropertyOf dc:description ;
        rdfs:isDefinedBy hxl:situationSection ;
        skos:prefLabel "situation description" ;
        rdfs:domain hxl:Situation ;
rdfs:range rdfs:Literal .

foaf:Agent
        a rdfs:Class , owl:Class ;
        rdfs:isDefinedBy hxl:situationSection  ;
skos:prefLabel "foaf:Agent" .

foaf:Organisation
        a rdfs:Class , owl:Class ;
        rdfs:isDefinedBy hxl:responseSection  ;
    skos:prefLabel "foaf:Organisation" ;
    rdfs:subClassOf foaf:Agent .

foaf:Group
        a rdfs:Class , owl:Class ;
        rdfs:isDefinedBy hxl:situationSection  ;
    skos:prefLabel "foaf:Group" ;
rdfs:subClassOf foaf:Agent .

hxl:featureName                                     #should this be a more generic property "name"?  Same question for featureAltName and featureRefName.
        a rdf:Property , owl:DataProperty ;        
        rdfs:isDefinedBy hxl:geolocationSection ;
        skos:prefLabel "feature name"@en ;
        rdfs:comment "The common name of the feature.  This is the accepted spelling of the name for the humanitarian community at the time of this version of the dataset."@en ;
        rdfs:domain hxl:Feature ;
rdfs:range rdfs:Literal .

hxl:featureAltName
        a rdf:Property , owl:DataProperty ;
        rdfs:isDefinedBy hxl:geolocationSection ;
        skos:prefLabel "feature alternate name"@en ;
        rdfs:comment "An alternative spelling of the feature.  This is not the accepted spelling of the name for the humanitarian community and should be avoided."@en ;
        rdfs:domain hxl:Feature ;
rdfs:range rdfs:Literal .

hxl:featureRefName
        a rdf:Property , owl:DataProperty ;
        rdfs:isDefinedBy hxl:geolocationSection ;
        skos:prefLabel "feature reference name"@en ;
        rdfs:comment "A version of the feature name in proper case without accented characters or apostrophes.  Spaces and hyphens are allowed."@en ;
        rdfs:domain hxl:Feature ;
rdfs:range rdfs:Literal .

hxl:version
        a rdf:Property , owl:ObjectProperty ;
        rdfs:isDefinedBy hxl:geolocationSection ;
        skos:prefLabel "dataset version"@en ;
        rdfs:comment "Specifies to which dataset version an admin unit belongs."@en ;
        rdfs:domain hxl:AdminUnit ;
rdfs:range hxl:AdminDatasetVersion .

hxl:AdminDatasetVersion
        a rdfs:Class ;
        rdfs:isDefinedBy hxl:geolocationSection ;
        skos:prefLabel "Administrative Units Dataset Version"@en ;
        rdfs:comment "Administrative Boundaries and Populated Places datasets form a hierarchical dataset that periodically changes.  The Administrative Units Dataset Version represents a complete set of these data valid for a particular period of time."@en .

hxl:validity
        a rdf:Property , owl:ObjectProperty ;
        rdfs:isDefinedBy hxl:geolocationSection ;
        skos:prefLabel "period of validity"@en ;
        rdfs:comment "The period of time in which a dataset was a valid reference."@en ;
        rdfs:domain hxl:AdminDatasetVersion ;
rdfs:range dc:PeriodOfTime .

hxl:adminDatasetVersionDescription
        a rdf:Property , owl:DataProperty ;
        rdfs:isDefinedBy hxl:geolocationSection ;
        skos:prefLabel "admin dataset version description"@en ;
        rdfs:comment "A description of a version of an administrative units dataset."@en ;
        rdfs:domain hxl:AdminDatasetVersion ;
rdfs:range rdfs:Literal .

hxl:versionID
        a rdf:Property , owl:DataProperty ;
        rdfs:isDefinedBy hxl:geolocationSection ;
        skos:prefLabel "version ID"@en ;
        rdfs:comment "Specifies the identifier for the Administrative Units Dataset."@en ;
        rdfs:domain hxl:AdminDatasetVersion ;
rdfs:range rdfs:Literal .

hxl:pcode
        a rdf:Property , owl:DataProperty ;
        rdfs:isDefinedBy hxl:geolocationSection ;
        skos:prefLabel "p-code"@en ;
        rdfs:comment "Specifies the unique identifier for an administrative unit or populated place.  This is the preferred way of referencing these geographic features."@en ;
        rdfs:domain hxl:AdminUnit ;
rdfs:range rdfs:Literal .

# Humanitarian Profile stuff added by CJ for Carsten's review

hxl:Intersex
        a rdfs:Class ;
        rdfs:isDefinedBy hxl:humanitarianProfileSection ;        
        skos:prefLabel "Intersex"@en;
        rdfs:subClassOf hxl:Sex ;
        rdfs:comment "A person or group of persons who are biologically intersex." ;
owl:disjointWith hxl:Female , hxl:Male , hxl:MixedSex .      # changes to disjoint property made for male and female also  

hxl:MixedSex
        a rdfs:Class ;
        rdfs:isDefinedBy hxl:humanitarianProfileSection ;
        skos:prefLabel "mixed sex"@en ;
        rdfs:subClassOf hxl:Sex ;
        rdfs:comment "A group of persons of mixed sexes."@en ;
owl:disjointWith hxl:Female , hxl:Male , hxl:Intersex . #changes to disjoint property for other sex categories also

hxl:sexCategory
        a rdf:Property , owl:ObjectProperty ;
        rdfs:isDefinedBy hxl:humanitarianProfileSection ;
        skos:prefLabel "sex category" ;
        rdfs:comment "Specifies the sex of the population." ;
        rdfs:domain hxl:Population ;
rdfs:range hxl:Sex .

#removed "rdfs:subClass foaf:Agent" from each of the four sex categories;

#removed "rdfs:subClass hxl:Population" from AgeGroup

hxl:AgeGroupSet
        a rdfs:Class ;
        rdfs:isDefinedBy hxl:humanitarianProfileSection ;
        skos:prefLabel "Age Group Set"@en ;
        rdfs:comment "Contains a set of bracketed age groups, usually defined as a standard by some authority."@en .
        
hxl:inAgeGroupSet
        a rdf:Property , owl:ObjectProperty ;
        rdfs:isDefinedBy hxl:humanitarianProfileSection ;
        skos:prefLabel "in age group set"@en ;
        rdfs:comment "Specifies to which Age Group Set a specific age group belongs." @en ;
        rdfs:domain hxl:AgeGroup ;
rdfs:range hxl:AgeGroupSet .

hxl:ageGroupSetTitle
        a rdf:Property , owl:DataProperty ;
        rdfs:isDefinedBy hxl:humanitarianProfileSection ;
        skos:prefLabel "age group set title"@en ;
        rdfs:comment "Specifies a title for an age group set."@en ;
        rdfs:domain hxl:AgeGroupSet ;
rdfs:range rdfs:Literal .

hxl:ageGroupSetDescription
        a rdf:Property , owl:DataProperty ;
        rdfs:isDefinedBy hxl:humanitarianProfileSection ;
        skos:prefLabel "age group set description"@en ;
        rdfs:comment "A description of a set of age groups. This should include a reference to the authority of the age group set."@en ;
        rdfs:domain hxl:AgeGroupSet ;
rdfs:range rdfs:Literal .

hxl:DisplacedLocationSetTitle
        a rdf:Property , owl:DataProperty ;
        rdfs:isDefinedBy hxl:humanitarianProfileSection ;
        skos:prefLabel "displaced persons location type set title"@en ;
        rdfs:comment "Specifies a title for a displaced persons location type set."@en ;
        rdfs:domain hxl:DisplacedLocationTypeSet ;
rdfs:range rdfs:Literal .

hxl:displacedLocationTypeSetDescription
        a rdf:Property , owl:DataProperty ;
        rdfs:isDefinedBy hxl:humanitarianProfileSection ;
        skos:prefLabel "displaced persons location type set description"@en ;
        rdfs:comment "A description of a set of Displaced Persons Location Types. This should include a reference to the authority of the set."@en ;
        rdfs:domain hxl:DisplacedLocationTypeSet ;
rdfs:range rdfs:Literal .

hxl:inDisplacedLocationType
        a rdf:Property , owl:ObjectProperty ;
        rdfs:isDefinedBy hxl:humanitarianProfileSection ;
        skos:prefLabel "in displaced location type"@en ;
        rdfs:comment "Specifies the type of living situation in which a population is living."@en ;
        rdfs:domain hxl:Displaced ;
rdfs:range hxl:DisplacedLocationTypeSet .

hxl:DisplacedLocationTypeSet
        a rdfs:Class ;
        rdfs:isDefinedBy hxl:humanitarianProfileSection ;
        skos:prefLabel "Displaced Persons Location Type Set"@en ;
        rdfs:comment "Generic class for classes describing the housing situation in which a displaced population is living. Subclasses of this class represent a coherent set of these location types which may vary from emergency to emergency.  The individual types are instances of the subclass."@en .

